Graph/Values.thy
@@ -19,8 +19,12 @@ currently allowed by our semantics, ranging from basic integer types
 to object references and arrays.
 
 Note that Java supports 64, 32, 16, 8 signed ints, plus 1 bit (boolean)
-ints, but during calculations the smaller sizes are sign-extended to 32 bits,
-so here we model just 32 and 64 bit values.
+ints, and char is 16-bit unsigned.
+E.g. an 8-bit stamp has a default range of -128..+127.
+And a 1-bit stamp has a default range of -1..0, surprisingly.
+
+During calculations the smaller sizes are sign-extended to 32 bits, but explicit 
+widening nodes will do that, so most binary calculations should see equal input sizes.
 
 An object reference is an option type where the @{term None} object reference
 points to the static fields. This is examined more closely in our
@@ -37,56 +41,102 @@ abbreviation valid_int_widths :: "nat set" where
   "valid_int_widths \<equiv> {1, 8, 16, 32, 64}"
 
 
+text \<open>Option 2: explicit width stored with each integer value.
+      However, this does not help us to distinguish between short (signed) and char (unsigned).\<close>
+
+typedef IntWidth = "{ w :: nat . w=1 \<or> w=8 \<or> w=16 \<or> w=32 \<or> w=64 }"
+  by blast
+
+setup_lifting type_definition_IntWidth
+
+lift_definition IntWidthBits :: "IntWidth \<Rightarrow> nat"
+  is "\<lambda>w. w" .
+
+
+text \<open>Option 3: explicit type stored with each integer value.\<close>
+
+datatype IntType = ILong | IInt | IShort | IChar | IByte | IBoolean
+
+fun int_bits :: "IntType \<Rightarrow> nat" where
+  "int_bits ILong  = 64" |
+  "int_bits IInt   = 32" |
+  "int_bits IShort = 16" |
+  "int_bits IChar  = 16" |
+  "int_bits IByte  =  8" |
+  "int_bits IBoolean = 1"
+
+fun int_signed :: "IntType \<Rightarrow> bool" where
+  "int_signed ILong  = True" |
+  "int_signed IInt   = True" |
+  "int_signed IShort = True" |
+  "int_signed IChar  = False" |
+  "int_signed IByte  =  True" |
+  "int_signed IBoolean = True"
+
+
+text \<open>Option 4: int64 with the number of significant bits.\<close>
+
+
+type_synonym iwidth = "nat"  (* TODO: 1..64 *)
 type_synonym objref = "nat option"
 
 datatype (discs_sels) Value  =
   UndefVal |
-  IntVal32 "32 word" |  (* also used for 16, 8, and 1-bit (boolean) values *)
-  IntVal64 "64 word" |
+  (* IntVal32 "32 word" | *)  (* also used for 16, 8, and 1-bit (boolean) values *)
+  (* IntVal64 "64 word" | *)
+  (* IntVal IntType int64 |  -- all types smaller than 64 bits are zero-extended *)
+  (* or widths: IntVal (ibits:IntWidth) (ival:int64) | *)
+  (* or just:   IntVal (ibits:nat) (ival:int64) ? *)
+  (* or         IntVal IntWord where IntWord = (nat,int64)? *)
+  (* IntValv2 nat bool int64 |   bits, signed, word *)
+  IntVal iwidth int64 | (* bits and word because we cannot know sign until do compare! *)
   (* FloatVal float | not supported *)
   ObjRef objref |
   ObjStr string
 
-text \<open>Characterise integer values, covering both 32 and 64 bit.
-  If a node has a stamp smaller than 32 bits (16, 8, or 1 bit),
-  then the value will be sign-extended to 32 bits.
-  This is necessary to match what the stamps specify 
-  E.g. an 8-bit stamp has a default range of -128..+127.
-  And a 1-bit stamp has a default range of -1..0, surprisingly.
-\<close>
+fun intval_bits :: "Value \<Rightarrow> nat" where
+  "intval_bits (IntVal b v) = b"
 
 definition logic_negate :: "('a::len) word \<Rightarrow> 'a word" where
   "logic_negate x = (if x = 0 then 1 else 0)"
 
-definition is_IntVal :: "Value \<Rightarrow> bool" where
-  "is_IntVal v = (is_IntVal32 v \<or> is_IntVal64 v)"
+fun int_signed_value :: "iwidth \<Rightarrow> int64 \<Rightarrow> int" where
+  "int_signed_value b v = sint (signed_take_bit (b - 1) v)"
 
-text \<open>Extract signed integer values from both 32 and 64 bit.\<close>
+fun int_unsigned_value :: "iwidth \<Rightarrow> int64 \<Rightarrow> int" where
+  "int_unsigned_value b v = uint (take_bit b v)"
 
-fun intval :: "Value \<Rightarrow> int" where
-  "intval (IntVal32 v) = sint v" |
-  "intval (IntVal64 v) = sint v"
+
+text \<open>Converts an integer word into a Java value.\<close>
+fun new_int :: "iwidth \<Rightarrow> int64 \<Rightarrow> Value" where
+  "new_int b w = IntVal b (take_bit b w)"
+
+text \<open>Converts an integer word into a Java value, iff the two types are equal.\<close>
+fun new_int_bin :: "iwidth \<Rightarrow> iwidth \<Rightarrow> int64 \<Rightarrow> Value" where
+  "new_int_bin b1 b2 w = (if b1=b2 then new_int b1 w else UndefVal)"
 
 
 fun wf_bool :: "Value \<Rightarrow> bool" where
-  "wf_bool (IntVal32 v) = (v = 0 \<or> v = 1)" |
+  "wf_bool (IntVal b w) = (b = 1)" |
   "wf_bool _ = False" 
 
 fun val_to_bool :: "Value \<Rightarrow> bool" where
-  "val_to_bool (IntVal32 val) = (if val = 0 then False else True)" |
-  "val_to_bool (IntVal64 val) = (if val = 0 then False else True)" |
-  "val_to_bool v = False"
+  "val_to_bool (IntVal b val) = (if val = 0 then False else True)" |
+  "val_to_bool val = False"
 
 fun bool_to_val :: "bool \<Rightarrow> Value" where
-  "bool_to_val True = (IntVal32 1)" |
-  "bool_to_val False = (IntVal32 0)"
+  "bool_to_val True = (IntVal 1 1)" |
+  "bool_to_val False = (IntVal 1 0)"
 
-value "sint(word_of_int (1) :: int1)"
 
+text \<open>Converts an Isabelle bool into a Java value, iff the two types are equal.\<close>
+fun bool_to_val_bin :: "iwidth \<Rightarrow> iwidth \<Rightarrow> bool \<Rightarrow> Value" where
+  "bool_to_val_bin t1 t2 b = (if t1 = t2 then bool_to_val b else UndefVal)"
+
+
+(* Deprecated - just for backwards compatibility. *)
 fun is_int_val :: "Value \<Rightarrow> bool" where
-  "is_int_val (IntVal32 v) = True" |
-  "is_int_val (IntVal64 v) = True" |
-  "is_int_val _ = False"
+  "is_int_val v = is_IntVal v"
 
 
 
@@ -102,17 +152,18 @@ The following collection of intval functions correspond to the JVM
 arithmetic operations.  We merge the 32 and 64 bit operations into
 a single function, even though the stamp of each IRNode tells us
 exactly what the bit widths will be.  These merged functions 
-know to make it easier to do the instantiation of Value as 'plus', etc.
+make it easier to do the instantiation of Value as 'plus', etc.
 It might be worse for reasoning, because it could cause more case analysis,
 but this does not seem to be a problem in practice.
 \<close>
 
 (* Corresponds to JVM iadd and ladd instructions. *)
 fun intval_add :: "Value \<Rightarrow> Value \<Rightarrow> Value" where
-  "intval_add (IntVal32 v1) (IntVal32 v2) = (IntVal32 (v1+v2))" |
-  "intval_add (IntVal64 v1) (IntVal64 v2) = (IntVal64 (v1+v2))" |
+  "intval_add (IntVal b1 v1) (IntVal b2 v2) = 
+    (if b1 = b2 then IntVal b1 (take_bit b1 (v1+v2)) else UndefVal)" |
   "intval_add _ _ = UndefVal"
 
+(* TODO if needed:
 instantiation Value :: ab_semigroup_add
 begin
 
@@ -126,19 +177,20 @@ instance proof
   show "a + b + c = a + (b + c)"
     apply (simp add: plus_Value_def)
     apply (induction a; induction b; induction c; auto)
-    done
+    
   show "a + b = b + a"
     apply (simp add: plus_Value_def)
     apply (induction a; induction b; auto)
     done
 qed
 end
+*)
 
 (* Corresponds to JVM isub and lsub instructions. *)
 fun intval_sub :: "Value \<Rightarrow> Value \<Rightarrow> Value" where
-  "intval_sub (IntVal32 v1) (IntVal32 v2) = (IntVal32 (v1-v2))" |
-  "intval_sub (IntVal64 v1) (IntVal64 v2) = (IntVal64 (v1-v2))" |
+  "intval_sub (IntVal b1 v1) (IntVal b2 v2) = new_int_bin b1 b2 (v1-v2)" |
   "intval_sub _ _ = UndefVal"
+
 
 instantiation Value :: minus
 begin
@@ -149,10 +201,10 @@ definition minus_Value :: "Value \<Rightarrow> Value \<Rightarrow> Value" where
 instance proof qed
 end
 
+
 (* Corresponds to JVM imul and lmul instructions. *)
 fun intval_mul :: "Value \<Rightarrow> Value \<Rightarrow> Value" where
-  "intval_mul (IntVal32 v1) (IntVal32 v2) = (IntVal32 (v1*v2))" |
-  "intval_mul (IntVal64 v1) (IntVal64 v2) = (IntVal64 (v1*v2))" |
+  "intval_mul (IntVal b1 v1) (IntVal b2 v2) = new_int_bin b1 b2 (v1*v2)" |
   "intval_mul _ _ = UndefVal"
 
 instantiation Value :: times
@@ -164,11 +216,13 @@ definition times_Value :: "Value \<Rightarrow> Value \<Rightarrow> Value" where
 instance proof qed
 end
 
+
 (* Java division rounds towards 0, so we use sdiv, not div. *)
 (* TODO: find a signed division operator in the Word library? *)
 fun intval_div :: "Value \<Rightarrow> Value \<Rightarrow> Value" where
-  "intval_div (IntVal32 v1) (IntVal32 v2) = (IntVal32 (word_of_int((sint v1) sdiv (sint v2))))" |
-  "intval_div (IntVal64 v1) (IntVal64 v2) = (IntVal64 (word_of_int((sint v1) sdiv (sint v2))))" |
+  "intval_div (IntVal b1 v1) (IntVal b2 v2) = 
+        new_int_bin b1 b2 (word_of_int
+           ((int_signed_value b1 v1) sdiv (int_signed_value b2 v2)))" |
   "intval_div _ _ = UndefVal"
 
 instantiation Value :: divide
@@ -182,11 +236,10 @@ end
 
 (* Java % is a modulo operator that can give negative results, since div rounds towards 0. *)
 fun intval_mod :: "Value \<Rightarrow> Value \<Rightarrow> Value" where
-  "intval_mod (IntVal32 v1) (IntVal32 v2) = (IntVal32 (word_of_int((sint v1) smod (sint v2))))" |
-  "intval_mod (IntVal64 v1) (IntVal64 v2) = (IntVal64 (word_of_int((sint v1) smod (sint v2))))" |
+  "intval_mod (IntVal b1 v1) (IntVal b2 v2) = 
+        new_int_bin b1 b2 (word_of_int
+           ((int_signed_value b1 v1) smod (int_signed_value b2 v2)))" |
   "intval_mod _ _ = UndefVal"
-  (* WAS: (IntVal 32 (sint((word_of_int(v1 smod v2) :: int32))))  *)
-  (*      (IntVal 64 (sint((word_of_int(v1 smod v2) :: int64)))))  *)
 
 instantiation Value :: modulo
 begin
@@ -209,73 +262,54 @@ begin
 
 
 fun intval_and :: "Value \<Rightarrow> Value \<Rightarrow> Value" where
-  "intval_and (IntVal32 v1) (IntVal32 v2) = (IntVal32 (v1 AND v2))" |
-  "intval_and (IntVal64 v1) (IntVal64 v2) = (IntVal64 (v1 AND v2))" |
+  "intval_and (IntVal b1 v1) (IntVal b2 v2) = new_int_bin b1 b2 (v1 AND v2)" |
   "intval_and _ _ = UndefVal"
 
 fun intval_or :: "Value \<Rightarrow> Value \<Rightarrow> Value" where
-  "intval_or (IntVal32 v1) (IntVal32 v2) = (IntVal32 (v1 OR v2))" |
-  "intval_or (IntVal64 v1) (IntVal64 v2) = (IntVal64 (v1 OR v2))" |
+  "intval_or (IntVal b1 v1) (IntVal b2 v2) = new_int_bin b1 b2 (v1 OR v2)" |
   "intval_or _ _ = UndefVal"
 
 fun intval_xor :: "Value \<Rightarrow> Value \<Rightarrow> Value" where
-  "intval_xor (IntVal32 v1) (IntVal32 v2) = (IntVal32 (v1 XOR v2))" |
-  "intval_xor (IntVal64 v1) (IntVal64 v2) = (IntVal64 (v1 XOR v2))" |
+  "intval_xor (IntVal b1 v1) (IntVal b2 v2) = new_int_bin b1 b2 (v1 XOR v2)" |
   "intval_xor _ _ = UndefVal"
 
 (* TODO: temp guess at semantics *)
 fun intval_short_circuit_or :: "Value \<Rightarrow> Value \<Rightarrow> Value" where
-  "intval_short_circuit_or (IntVal32 v1) (IntVal32 v2) = (IntVal32 (v1 OR v2))" |
-  "intval_short_circuit_or (IntVal64 v1) (IntVal64 v2) = (IntVal64 (v1 OR v2))" |
+  "intval_short_circuit_or (IntVal b1 v1) (IntVal b2 v2) = new_int_bin b1 b2 (v1 OR v2)" |
   "intval_short_circuit_or _ _ = UndefVal"
 
 fun intval_equals :: "Value \<Rightarrow> Value \<Rightarrow> Value" where
-  "intval_equals (IntVal32 v1) (IntVal32 v2) = bool_to_val (v1 = v2)" |
-  "intval_equals (IntVal64 v1) (IntVal64 v2) = bool_to_val (v1 = v2)" |
+  "intval_equals (IntVal b1 v1) (IntVal b2 v2) = bool_to_val_bin b1 b2 (v1 = v2)" |
   "intval_equals _ _ = UndefVal"
 
 fun intval_less_than :: "Value \<Rightarrow> Value \<Rightarrow> Value" where
-  "intval_less_than (IntVal32 v1) (IntVal32 v2) = bool_to_val (v1 <s v2)" |
-  "intval_less_than (IntVal64 v1) (IntVal64 v2) = bool_to_val (v1 <s v2)" |
+  "intval_less_than (IntVal b1 v1) (IntVal b2 v2) = 
+    bool_to_val_bin b1 b2 (int_signed_value b1 v1 < int_signed_value b2 v2)" |
   "intval_less_than _ _ = UndefVal"
 
 fun intval_below :: "Value \<Rightarrow> Value \<Rightarrow> Value" where
-  "intval_below (IntVal32 v1) (IntVal32 v2) = bool_to_val (v1 < v2)" |
-  "intval_below (IntVal64 v1) (IntVal64 v2) = bool_to_val (v1 < v2)" |
+  "intval_below (IntVal b1 v1) (IntVal b2 v2) = bool_to_val_bin b1 b2 (v1 < v2)" |
   "intval_below _ _ = UndefVal"
 
 fun intval_not :: "Value \<Rightarrow> Value" where
-  "intval_not (IntVal32 v) = (IntVal32 (NOT v))" |
-  "intval_not (IntVal64 v) = (IntVal64 (NOT v))" |
+  "intval_not (IntVal t v) = new_int t (NOT v)" |
   "intval_not _ = UndefVal"
 
 fun intval_negate :: "Value \<Rightarrow> Value" where
-  "intval_negate (IntVal32 v) = IntVal32 (- v)" |
-  "intval_negate (IntVal64 v) = IntVal64 (- v)" |
+  "intval_negate (IntVal t v) = new_int t (- v)" |
   "intval_negate _ = UndefVal"
 
 fun intval_abs :: "Value \<Rightarrow> Value" where
-  "intval_abs (IntVal32 v) = (if (v) <s 0 then (IntVal32 (- v)) else (IntVal32 v))" |
-  "intval_abs (IntVal64 v) = (if (v) <s 0 then (IntVal64 (- v)) else (IntVal64 v))" |
+  "intval_abs (IntVal t v) = new_int t (if int_signed_value t v < 0 then - v else v)" |
   "intval_abs _ = UndefVal"
 
 fun intval_conditional :: "Value \<Rightarrow> Value \<Rightarrow> Value \<Rightarrow> Value" where
   "intval_conditional cond tv fv = (if (val_to_bool cond) then tv else fv)"
 
+text \<open>TODO: clarify which widths this should work on: just 1-bit or all?\<close>
 fun intval_logic_negation :: "Value \<Rightarrow> Value" where
-  "intval_logic_negation (IntVal32 v) = (IntVal32 (logic_negate v))" |
-  "intval_logic_negation (IntVal64 v) = (IntVal64 (logic_negate v))" |
+  "intval_logic_negation (IntVal b v) = (IntVal b (logic_negate v))" |
   "intval_logic_negation _ = UndefVal"
-
-lemma intval_eq32:
-  assumes "intval_equals (IntVal32 v1) v2 \<noteq> UndefVal"
-  shows "is_IntVal32 v2"
-  by (metis Value.exhaust_disc assms intval_equals.simps(10) intval_equals.simps(12) intval_equals.simps(15) intval_equals.simps(16) is_IntVal64_def is_ObjRef_def is_ObjStr_def)
-
-lemma intval_eq32_simp:
-  assumes "intval_equals (IntVal32 v1) v2 \<noteq> UndefVal"
-  shows "intval_equals (IntVal32 v1) v2 = bool_to_val (v1 = un_IntVal32 v2)"
-  by (metis Value.collapse(1) assms intval_eq32 intval_equals.simps(1))
 
 
 
@@ -284,9 +318,7 @@ subsection \<open>Narrowing and Widening Operators\<close>
 text \<open>Note: we allow these operators to have inBits=outBits, because the Graal compiler
   also seems to allow that case, even though it should rarely / never arise in practice.\<close>
 
-text \<open>When narrowing to less than 32 bits, we sign extend back to 32 bits,
-  because we always represent integer values as either 32 or 64 bits.\<close>
-
+(* Not needed now:
 fun narrow_helper :: "nat \<Rightarrow> nat \<Rightarrow> int32 \<Rightarrow> Value" where
   "narrow_helper inBits outBits val =
     (if outBits \<le> inBits \<and> outBits \<le> 32 \<and>
@@ -294,30 +326,27 @@ fun narrow_helper :: "nat \<Rightarrow> nat \<Rightarrow> int32 \<Rightarrow> Va
         inBits \<in> valid_int_widths
      then IntVal32 (signed_take_bit (outBits - 1) val)
      else UndefVal)"
+*)
 
 value "sint(signed_take_bit 0 (1 :: int32))" (* gives -1, which matches compiler *)
 
 fun intval_narrow :: "nat \<Rightarrow> nat \<Rightarrow> Value \<Rightarrow> Value" where
-  "intval_narrow inBits outBits (IntVal32 v) =
-     (if inBits = 64 
-      then UndefVal
-      else narrow_helper inBits outBits v)" |
-  "intval_narrow inBits outBits (IntVal64 v) = 
-     (if inBits = 64 
-      then (if outBits = 64 
-            then IntVal64 v 
-            else narrow_helper inBits outBits (scast v))
+  "intval_narrow inBits outBits (IntVal b v) =
+     (if inBits = b \<and> outBits \<le> inBits  
+      then new_int outBits v
       else UndefVal)" |
   "intval_narrow _ _ _ = UndefVal"
 
 value "intval(intval_narrow 16 8 (IntVal32 (512 - 2)))"  (* gives -2 (IntVal32 4294967294) *)
 
-
+(* Not needed now:
 fun choose_32_64 :: "nat \<Rightarrow> int64 \<Rightarrow> Value" where
   "choose_32_64 outBits v = (if outBits = 64 then (IntVal64 v) else (IntVal32 (scast v)))"
+*)
 
 value "sint (signed_take_bit 7 ((256 + 128) :: int64))"
 
+(*
 fun sign_extend_helper :: "nat \<Rightarrow> nat \<Rightarrow> int32 \<Rightarrow> Value" where
   "sign_extend_helper inBits outBits val =
     (if inBits \<le> outBits \<and> inBits \<le> 32 \<and>
@@ -328,16 +357,16 @@ fun sign_extend_helper :: "nat \<Rightarrow> nat \<Rightarrow> int32 \<Rightarro
         then IntVal64 (scast (signed_take_bit (inBits - 1) val))
         else IntVal32 (signed_take_bit (inBits - 1) val))
      else UndefVal)"
-
+*)
 
 fun intval_sign_extend :: "nat \<Rightarrow> nat \<Rightarrow> Value \<Rightarrow> Value" where
-  "intval_sign_extend inBits outBits (IntVal32 v) =
-     sign_extend_helper inBits outBits v" |
-  "intval_sign_extend inBits outBits (IntVal64 v) = 
-     (if inBits=64 \<and> outBits=64 then IntVal64 v else UndefVal)" |
+  "intval_sign_extend inBits outBits (IntVal b v) =
+     (if inBits = b \<and> outBits \<ge> inBits  
+      then new_int outBits (signed_take_bit (inBits - 1) v)
+      else UndefVal)" |
   "intval_sign_extend _ _ _ = UndefVal"
 
-
+(* Not needed now:
 fun zero_extend_helper :: "nat \<Rightarrow> nat \<Rightarrow> int32 \<Rightarrow> Value" where
   "zero_extend_helper inBits outBits val =
     (if inBits \<le> outBits \<and> inBits \<le> 32 \<and>
@@ -348,34 +377,28 @@ fun zero_extend_helper :: "nat \<Rightarrow> nat \<Rightarrow> int32 \<Rightarro
         then IntVal64 (ucast (take_bit inBits val))
         else IntVal32 (take_bit inBits val))
      else UndefVal)"
+*)
 
 fun intval_zero_extend :: "nat \<Rightarrow> nat \<Rightarrow> Value \<Rightarrow> Value" where
-  "intval_zero_extend inBits outBits (IntVal32 v) =
-     zero_extend_helper inBits outBits v" |
-  "intval_zero_extend inBits outBits (IntVal64 v) = 
-     (if inBits=64 \<and> outBits=64 then IntVal64 v else UndefVal)" |
+  "intval_zero_extend inBits outBits (IntVal b v) =
+     (if inBits = b \<and> outBits \<ge> inBits  
+      then new_int outBits (take_bit inBits v)
+      else UndefVal)" |
   "intval_zero_extend _ _ _ = UndefVal"
 
 
 text \<open>Some well-formedness results to help reasoning about narrowing and widening operators\<close>
 
-lemma narrow_helper_ok:
-  assumes "narrow_helper inBits outBits val \<noteq> UndefVal"
-  shows "0 < outBits \<and> outBits \<le> 32 \<and>
-        outBits \<le> inBits \<and>
-        outBits \<in> valid_int_widths \<and>
-        inBits \<in> valid_int_widths"
-  using assms narrow_helper.simps neq0_conv by fastforce
-
 lemma intval_narrow_ok:
   assumes "intval_narrow inBits outBits val \<noteq> UndefVal"
-  shows "0 < outBits \<and>
+  shows "0 \<le> outBits \<and>
         outBits \<le> inBits \<and> 
-        outBits \<in> valid_int_widths \<and>
-        inBits \<in> valid_int_widths"
-  using assms narrow_helper_ok intval_narrow.simps neq0_conv
-  by (smt (verit, best) insertCI intval_sign_extend.elims order_le_less zero_neq_numeral) 
+        is_IntVal val \<and>
+        intval_bits val = inBits"
+  using assms intval_narrow.simps neq0_conv intval_bits.simps
+  by (metis intval_narrow.elims is_IntVal_def less_eq_nat.simps(1))
 
+(* Not needed now:
 lemma narrow_takes_64:
   assumes "result = intval_narrow inBits outBits value"
   assumes "result \<noteq> UndefVal"
@@ -389,7 +412,6 @@ lemma narrow_gives_64:
   using assms
   by (smt (verit, best) Value.case_eq_if Value.discI(1) Value.discI(2) Value.disc_eq_case(3) add_diff_cancel_left' diff_is_0_eq intval_narrow.elims narrow_helper.simps numeral_Bit0 zero_neq_numeral) 
 
-
 lemma sign_extend_helper_ok:
   assumes "sign_extend_helper inBits outBits val \<noteq> UndefVal"
   shows "0 < inBits \<and> inBits \<le> 32 \<and>
@@ -397,16 +419,18 @@ lemma sign_extend_helper_ok:
         outBits \<in> valid_int_widths \<and>
         inBits \<in> valid_int_widths"
   using assms sign_extend_helper.simps neq0_conv by fastforce
+*)
 
 lemma intval_sign_extend_ok:
   assumes "intval_sign_extend inBits outBits val \<noteq> UndefVal"
-  shows "0 < inBits \<and>
+  shows "0 \<le> inBits \<and>
         inBits \<le> outBits \<and> 
-        outBits \<in> valid_int_widths \<and>
-        inBits \<in> valid_int_widths"
-  using assms sign_extend_helper_ok intval_sign_extend.simps neq0_conv
-  by (smt (verit, best) insertCI intval_sign_extend.elims order_le_less zero_neq_numeral) 
+        is_IntVal val \<and>
+        intval_bits val = inBits"
+  using assms intval_sign_extend.simps neq0_conv
+  by (metis intval_bits.simps intval_sign_extend.elims is_IntVal_def less_eq_nat.simps(1))
 
+(*
 lemma zero_extend_helper_ok:
   assumes "zero_extend_helper inBits outBits val \<noteq> UndefVal"
   shows "0 < inBits \<and> inBits \<le> 32 \<and>
@@ -414,16 +438,16 @@ lemma zero_extend_helper_ok:
         outBits \<in> valid_int_widths \<and>
         inBits \<in> valid_int_widths"
   using assms zero_extend_helper.simps neq0_conv by fastforce
+*)
 
 lemma intval_zero_extend_ok:
   assumes "intval_zero_extend inBits outBits val \<noteq> UndefVal"
-  shows "0 < inBits \<and>
+  shows "0 \<le> inBits \<and>
         inBits \<le> outBits \<and> 
-        outBits \<in> valid_int_widths \<and>
-        inBits \<in> valid_int_widths"
-  using assms zero_extend_helper_ok intval_zero_extend.simps neq0_conv
-  by (smt (verit, best) insertCI intval_zero_extend.elims order_le_less zero_neq_numeral) 
-
+        is_IntVal val \<and>
+        intval_bits val = inBits"
+  using assms intval_sign_extend.simps neq0_conv
+  by (metis intval_bits.simps intval_zero_extend.elims is_IntVal_def less_eq_nat.simps(1))
 
 
 subsection \<open>Bit-Shifting Operators\<close>
@@ -474,25 +498,26 @@ text \<open>Note that Java shift operators use unary numeric promotion, unlike o
   This means that the left-hand input determines the output size, while the 
   right-hand input can be any size.\<close>
 
+fun shift_amount :: "iwidth \<Rightarrow> int64 \<Rightarrow> nat" where
+  "shift_amount b val = unat (val AND (if b = 64 then 0x3F else 0x1f))"
+
 fun intval_left_shift :: "Value \<Rightarrow> Value \<Rightarrow> Value" where
-  "intval_left_shift (IntVal32 v1) (IntVal32 v2) = IntVal32 (v1 << unat (v2 AND 0x1f))" |
-  "intval_left_shift (IntVal32 v1) (IntVal64 v2) = IntVal32 (v1 << unat (v2 AND 0x1f))" |
-  "intval_left_shift (IntVal64 v1) (IntVal32 v2) = IntVal64 (v1 << unat (v2 AND 0x3f))" |
-  "intval_left_shift (IntVal64 v1) (IntVal64 v2) = IntVal64 (v1 << unat (v2 AND 0x3f))" |
+  "intval_left_shift (IntVal b1 v1) (IntVal b2 v2) = new_int b1 (v1 << shift_amount b1 v2)" |
   "intval_left_shift _ _ = UndefVal"
 
+text \<open>Signed shift is more complex, because we sometimes have to insert 1 bits
+  at the correct point, which is at b1 bits.\<close>
 fun intval_right_shift :: "Value \<Rightarrow> Value \<Rightarrow> Value" where
-  "intval_right_shift (IntVal32 v1) (IntVal32 v2) = IntVal32 (v1 >> unat (v2 AND 0x1f))" |
-  "intval_right_shift (IntVal32 v1) (IntVal64 v2) = IntVal32 (v1 >> unat (v2 AND 0x1f))" |
-  "intval_right_shift (IntVal64 v1) (IntVal32 v2) = IntVal64 (v1 >> unat (v2 AND 0x3f))" |
-  "intval_right_shift (IntVal64 v1) (IntVal64 v2) = IntVal64 (v1 >> unat (v2 AND 0x3f))" |
+  "intval_right_shift (IntVal b1 v1) (IntVal b2 v2) = 
+     (let shift = shift_amount b1 v2 in
+      let ones = mask b1 AND (NOT (mask (b1 - shift) :: int64)) in
+      (if int_signed_value b1 v1 < 0
+       then new_int b1 (ones OR (v1 >>> shift))
+       else new_int b1 (v1 >>> shift)))" |
   "intval_right_shift _ _ = UndefVal"
 
 fun intval_uright_shift :: "Value \<Rightarrow> Value \<Rightarrow> Value" where
-  "intval_uright_shift (IntVal32 v1) (IntVal32 v2) = IntVal32 (v1 >>> unat (v2 AND 0x1f))" |
-  "intval_uright_shift (IntVal32 v1) (IntVal64 v2) = IntVal32 (v1 >>> unat (v2 AND 0x1f))" |
-  "intval_uright_shift (IntVal64 v1) (IntVal32 v2) = IntVal64 (v1 >>> unat (v2 AND 0x3f))" |
-  "intval_uright_shift (IntVal64 v1) (IntVal64 v2) = IntVal64 (v1 >>> unat (v2 AND 0x3f))" |
+  "intval_uright_shift (IntVal b1 v1) (IntVal b2 v2) = new_int b1 (v1 >>> shift_amount b1 v2)" |
   "intval_uright_shift _ _ = UndefVal"
 
 end
@@ -501,48 +526,55 @@ end
 section \<open>Examples of Narrowing / Widening Functions\<close>
 
 experiment begin
-corollary "intval_narrow 32 8 (IntVal32 (256 + 128)) = IntVal32 (-128)" by simp
-corollary "intval_narrow 32 8 (IntVal32 (-2)) = IntVal32 (-2)" by simp
-corollary "intval_narrow 32 1 (IntVal32 (-2)) = IntVal32 0"    by simp
-corollary "intval_narrow 32 1 (IntVal32 (-3)) = IntVal32 (-1)" by simp
+corollary "intval_narrow 32 8 (IntVal 32 (256 + 128)) = IntVal 8 128" by simp
+corollary "intval_narrow 32 8 (IntVal 32 (-2)) = IntVal 8 254" by simp
+corollary "intval_narrow 32 1 (IntVal 32 (-2)) = IntVal 1 0"    by simp
+corollary "intval_narrow 32 1 (IntVal 32 (-3)) = IntVal 1 1" by simp
 
 (* now test some 64 bit inputs and outputs *)
-corollary "intval_narrow 32 8 (IntVal64 (-2)) = UndefVal" by simp
-corollary "intval_narrow 64 8 (IntVal32 (-2)) = UndefVal" by simp
-corollary "intval_narrow 64 8 (IntVal64 (-2)) = IntVal32 (-2)" by simp
-corollary "intval_narrow 64 8 (IntVal64 (256+127)) = IntVal32 127" by simp
-corollary "intval_narrow 64 32 (IntVal64 (-2)) = IntVal32 (-2)" by simp
-corollary "intval_narrow 64 64 (IntVal64 (-2)) = IntVal64 (-2)" by simp
+corollary "intval_narrow 32 8 (IntVal 64 (-2)) = UndefVal" by simp
+corollary "intval_narrow 64 8 (IntVal 32 (-2)) = UndefVal" by simp
+corollary "intval_narrow 64 8 (IntVal 64 254) = IntVal 8 254" by simp
+corollary "intval_narrow 64 8 (IntVal 64 (256+127)) = IntVal 8 127" by simp
+corollary "intval_narrow 64 64 (IntVal 64 (-2)) = IntVal 64 (-2)" by simp
 end
 
 experiment begin
-corollary "intval_sign_extend 8 32 (IntVal32 (256 + 128)) = IntVal32 (-128)" by simp
-corollary "intval_sign_extend 8 32 (IntVal32 (-2)) = IntVal32 (-2)" by simp
-corollary "intval_sign_extend 1 32 (IntVal32 (-2)) = IntVal32 0"    by simp
-corollary "intval_sign_extend 1 32 (IntVal32 (-3)) = IntVal32 (-1)" by simp
+corollary "intval_sign_extend 8 32 (IntVal 8 (256 + 128)) = IntVal 32 (2^32 - 128)" by simp
+corollary "intval_sign_extend 8 32 (IntVal 8 (-2)) = IntVal 32 (2^32 - 2)" by simp
+corollary "intval_sign_extend 1 32 (IntVal 1 (-2)) = IntVal 32 0"    by simp
+corollary "intval_sign_extend 1 32 (IntVal 1 (-3)) = IntVal 32 (mask 32)" by simp
 
 (* now test some 64 bit inputs and outputs *)
-corollary "intval_sign_extend 8 32 (IntVal64 (-2)) = UndefVal" by simp
-corollary "intval_sign_extend 8 64 (IntVal64 (-2)) = UndefVal" by simp
-corollary "intval_sign_extend 8 64 (IntVal32 (-2)) = IntVal64 (-2)" by simp
-corollary "intval_sign_extend 32 64 (IntVal32 (-2)) = IntVal64 (-2)" by simp
-corollary "intval_sign_extend 64 64 (IntVal64 (-2)) = IntVal64 (-2)" by simp
+corollary "intval_sign_extend 8 32 (IntVal 64 254) = UndefVal" by simp
+corollary "intval_sign_extend 8 64 (IntVal 32 254) = UndefVal" by simp
+corollary "intval_sign_extend 8 64 (IntVal 8 254) = IntVal 64 (-2)" by simp
+corollary "intval_sign_extend 32 64 (IntVal 32 (2^32 - 2)) = IntVal 64 (-2)" by simp
+corollary "intval_sign_extend 64 64 (IntVal 64 (-2)) = IntVal 64 (-2)" by simp
 end
 
 
 experiment begin
-corollary "intval_zero_extend 8 32 (IntVal32 (256 + 128)) = IntVal32 128" by simp
-corollary "intval_zero_extend 8 32 (IntVal32 (-2)) = IntVal32 254" by simp
-corollary "intval_zero_extend 1 32 (IntVal32 (-1)) = IntVal32 1"   by simp
-corollary "intval_zero_extend 1 32 (IntVal32 (-2)) = IntVal32 0"   by simp
+corollary "intval_zero_extend 8 32 (IntVal 8 (256 + 128)) = IntVal 32 128" by simp
+corollary "intval_zero_extend 8 32 (IntVal 8 (-2)) = IntVal 32 254" by simp
+corollary "intval_zero_extend 1 32 (IntVal 1 (-1)) = IntVal 32 1"   by simp
+corollary "intval_zero_extend 1 32 (IntVal 1 (-2)) = IntVal 32 0"   by simp
 
 (* now test some 64 bit inputs and outputs *)
-corollary "intval_zero_extend 8 32 (IntVal64 (-2)) = UndefVal" by simp
-corollary "intval_zero_extend 8 64 (IntVal64 (-2)) = UndefVal" by simp
-corollary "intval_zero_extend 8 64 (IntVal32 (-2)) = IntVal64 254" by simp
-corollary "intval_zero_extend 32 64 (IntVal32 (-2)) = IntVal64 4294967294" by simp
+corollary "intval_zero_extend 8 32 (IntVal 64 (-2)) = UndefVal" by simp
+corollary "intval_zero_extend 8 64 (IntVal 64 (-2)) = UndefVal" by simp
+corollary "intval_zero_extend 8 64 (IntVal 8 254) = IntVal 64 254" by simp
+corollary "intval_zero_extend 32 64 (IntVal 32 (2^32 - 2)) = IntVal 64 (2^32 - 2)" by simp
+corollary "intval_zero_extend 64 64 (IntVal 64 (-2)) = IntVal 64 (-2)" by simp
 end
 
+experiment begin
+corollary "intval_right_shift (IntVal 8 128) (IntVal 8 0) = IntVal 8 128" by eval
+corollary "intval_right_shift (IntVal 8 128) (IntVal 8 1) = IntVal 8 192" by eval
+corollary "intval_right_shift (IntVal 8 128) (IntVal 8 2) = IntVal 8 224" by eval
+corollary "intval_right_shift (IntVal 8 128) (IntVal 8 8) = IntVal 8 255" by eval
+corollary "intval_right_shift (IntVal 8 128) (IntVal 8 31) = IntVal 8 255" by eval
+end
 
 (* ========================================================================
    Commutative and Associative results.  (Not used yet).
@@ -551,7 +583,7 @@ end
 (* commutative rules to be used when needed. *)
 lemma intval_add_sym:
   shows "intval_add a b = intval_add b a"
-  by (induction a; induction b; auto)
+  by (induction a; induction b; auto simp: add.commute)
 
 
 code_deps intval_add  (* view dependency graph of code definitions *)
@@ -559,9 +591,9 @@ code_thms intval_add  (* print all code definitions used by intval_add *)
 
 
 (* Some example tests. *)
-lemma "intval_add (IntVal32 (2^31-1)) (IntVal32 (2^31-1)) = IntVal32 (-2)"
+lemma "intval_add (IntVal 32 (2^31-1)) (IntVal 32 (2^31-1)) = IntVal 32 (2^32 - 2)"
   by eval
-lemma "intval_add (IntVal64 (2^31-1)) (IntVal64 (2^31-1)) = IntVal64 4294967294"
+lemma "intval_add (IntVal 64 (2^31-1)) (IntVal 64 (2^31-1)) = IntVal 64 4294967294"
   by eval
 
 end
